Generalized binding syntax overhaul: only two new binders: `() and `{}, guessing the binding name by default and making all generalized variables implicit. At the same time, continue refactoring of Record/Class/Inductive etc.., getting rid of [VernacRecord] definitively. The AST is not completely satisfying, but leaning towards Record/Class as restrictions of inductive (Arnaud, anyone ?). Now, [Class] declaration bodies are either of the form [meth : type] or [{ meth : type ; ... }], distinguishing singleton "definitional" classes and inductive classes based on records. The constructor syntax is accepted ([meth1 : type1 | meth1 : type2]) but raises an error immediately, as support for defining a class by a general inductive type is not there yet (this is a bugfix!).
git-svn-id: svn+ssh://scm.gforge.inria.fr/svn/coq/trunk@11679 85f007b7-540e-0410-9357-904b9bb8a0f7

contrib/funind/rawterm_to_relation.ml
@@ -1370,7 +1370,7 @@ let do_build_inductive
 	let _time3 = System.get_time () in
 (* 	Pp.msgnl (str "error : "++ str (string_of_float (System.time_difference time2 time3))); *)
 	let repacked_rel_inds = 
-	  List.map  (fun ((a , b , c , l),ntn) -> (a , b, c , Vernacexpr.Constructors l),ntn )
+	  List.map  (fun ((a , b , c , l),ntn) -> ((false,a) , b, c , None, Vernacexpr.Constructors l),ntn )
 	                  rel_inds
 	in
 	let msg = 		     
@@ -1385,7 +1385,7 @@ let do_build_inductive
 	let _time3 = System.get_time () in
 (* 	Pp.msgnl (str "error : "++ str (string_of_float (System.time_difference time2 time3))); *)
 	let repacked_rel_inds = 
-	  List.map  (fun ((a , b , c , l),ntn) -> (a , b, c , Vernacexpr.Constructors l),ntn )
+	  List.map  (fun ((a , b , c , l),ntn) -> ((false,a) , b, c , None, Vernacexpr.Constructors l),ntn )
 	                  rel_inds
 	in
 	let msg = 		     
