contrib/subtac/subtac_classes.ml
@@ -137,7 +137,9 @@ let new_instance ?(global=false) ctx (instid, bk, cl) props ?(generalize=true) p
   let sigma = Evd.evars_of !isevars in
   let subst = List.map (Evarutil.nf_evar sigma) subst in
   let subst = 
-    let props = match props with CRecord (loc, _, fs) -> fs | _ -> assert false in
+    let props = match props with CRecord (loc, _, fs) -> fs
+      | _ -> errorlabstrm "new_instance" (Pp.str "Expected a record declaration for the instance body") 
+    in
       if List.length props > List.length k.cl_props then 
 	Classes.mismatched_props env' (List.map snd props) k.cl_props;
       match k.cl_props with 
