theories/Classes/SetoidClass.v
@@ -26,9 +26,9 @@ Require Import Coq.Classes.Functions.
 
 (** A setoid wraps an equivalence. *)
 
-Class Setoid A :=
+Class Setoid A := {
   equiv : relation A ;
-  setoid_equiv :> Equivalence equiv.
+  setoid_equiv :> Equivalence equiv }.
 
 (* Too dangerous instance *)
 (* Program Instance [ eqa : Equivalence A eqA ] =>  *)
@@ -37,13 +37,13 @@ Class Setoid A :=
 
 (** Shortcuts to make proof search easier. *)
 
-Definition setoid_refl [ sa : Setoid A ] : Reflexive equiv.
+Definition setoid_refl `(sa : Setoid A) : Reflexive equiv.
 Proof. typeclasses eauto. Qed.
 
-Definition setoid_sym [ sa : Setoid A ] : Symmetric equiv.
+Definition setoid_sym `(sa : Setoid A) : Symmetric equiv.
 Proof. typeclasses eauto. Qed.
 
-Definition setoid_trans [ sa : Setoid A ] : Transitive equiv.
+Definition setoid_trans `(sa : Setoid A) : Transitive equiv.
 Proof. typeclasses eauto. Qed.
 
 Existing Instance setoid_refl.
@@ -55,7 +55,7 @@ Existing Instance setoid_trans.
 (* Program Instance eq_setoid : Setoid A := *)
 (*   equiv := eq ; setoid_equiv := eq_equivalence. *)
 
-Program Instance iff_setoid : Setoid Prop :=
+Program Instance iff_setoid : Setoid Prop := 
   equiv := iff ; setoid_equiv := iff_equivalence.
 
 (** Overloaded notations for setoid equivalence and inequivalence. Not to be confused with [eq] and [=]. *)
@@ -84,7 +84,7 @@ Ltac clsubst_nofail :=
 
 Tactic Notation "clsubst" "*" := clsubst_nofail.
 
-Lemma nequiv_equiv_trans : forall [ Setoid A ] (x y z : A), x =/= y -> y == z -> x =/= z.
+Lemma nequiv_equiv_trans : forall `{Setoid A} (x y z : A), x =/= y -> y == z -> x =/= z.
 Proof with auto.
   intros; intro.
   assert(z == y) by (symmetry ; auto).
@@ -92,7 +92,7 @@ Proof with auto.
   contradiction.
 Qed.
 
-Lemma equiv_nequiv_trans : forall [ Setoid A ] (x y z : A), x == y -> y =/= z -> x =/= z.
+Lemma equiv_nequiv_trans : forall `{Setoid A} (x y z : A), x == y -> y =/= z -> x =/= z.
 Proof.
   intros; intro. 
   assert(y == x) by (symmetry ; auto).
@@ -119,18 +119,11 @@ Ltac setoidify := repeat setoidify_tac.
 
 (** Every setoid relation gives rise to a morphism, in fact every partial setoid does. *)
 
-Program Definition setoid_morphism [ sa : Setoid A ] : Morphism (equiv ++> equiv ++> iff) equiv :=
-  PER_morphism.
+Program Instance setoid_morphism `(sa : Setoid A) : Morphism (equiv ++> equiv ++> iff) equiv :=
+  respect := respect.
 
-(** Add this very useful instance in the database. *)
-
-Implicit Arguments setoid_morphism [[!sa]].
-Existing Instance setoid_morphism.
-
-Program Definition setoid_partial_app_morphism [ sa : Setoid A ] (x : A) : Morphism (equiv ++> iff) (equiv x) :=
-  Reflexive_partial_app_morphism.
-
-Existing Instance setoid_partial_app_morphism.
+Program Instance setoid_partial_app_morphism `(sa : Setoid A) (x : A) : Morphism (equiv ++> iff) (equiv x) :=
+  respect := respect.
 
 Ltac morphism_tac := try red ; unfold arrow ; intros ; program_simpl ; try tauto.
 
@@ -144,9 +137,8 @@ Program Instance iff_impl_id_morphism : Morphism (iff ++> impl) id.
 
 (** Partial setoids don't require reflexivity so we can build a partial setoid on the function space. *)
 
-Class PartialSetoid (A : Type) :=
-  pequiv : relation A ;
-  pequiv_prf :> PER pequiv.
+Class PartialSetoid (A : Type) := 
+  { pequiv : relation A ; pequiv_prf :> PER pequiv }.
 
 (** Overloaded notation for partial setoid equivalence. *)
 
